theories/heap_lang/lifting.v
@@ -18,7 +18,7 @@ Instance heapG_irisG `{heapG Σ} : irisG heap_lang Σ := {
   iris_invG := heapG_invG;
   state_interp σ κs _ :=
     (gen_heap_ctx σ.(heap) ∗ proph_map_ctx κs σ.(used_proph_id))%I;
-  fork_post := True%I;
+  fork_post _ := True%I;
 }.
 
 (** Override the notations so that scopes and coercions work out *)
