theories/program_logic/ectx_lifting.v
@@ -21,7 +21,7 @@ Lemma wp_lift_head_step_fupd {s E Φ} e1 :
     ∀ e2 σ2 efs, ⌜head_step e1 σ1 κ e2 σ2 efs⌝ ={∅,∅,E}▷=∗
       state_interp σ2 κs (length efs + n) ∗
       WP e2 @ s; E {{ Φ }} ∗
-      [∗ list] ef ∈ efs, WP ef @ s; ⊤ {{ _, fork_post }})
+      [∗ list] ef ∈ efs, WP ef @ s; ⊤ {{ fork_post }})
   ⊢ WP e1 @ s; E {{ Φ }}.
 Proof.
   iIntros (?) "H". iApply wp_lift_step_fupd=>//. iIntros (σ1 κ κs Qs) "Hσ".
@@ -37,7 +37,7 @@ Lemma wp_lift_head_step {s E Φ} e1 :
     ▷ ∀ e2 σ2 efs, ⌜head_step e1 σ1 κ e2 σ2 efs⌝ ={∅,E}=∗
       state_interp σ2 κs (length efs + n) ∗
       WP e2 @ s; E {{ Φ }} ∗
-      [∗ list] ef ∈ efs, WP ef @ s; ⊤ {{ _, fork_post }})
+      [∗ list] ef ∈ efs, WP ef @ s; ⊤ {{ fork_post }})
   ⊢ WP e1 @ s; E {{ Φ }}.
 Proof.
   iIntros (?) "H". iApply wp_lift_head_step_fupd; [done|]. iIntros (????) "?".
@@ -72,7 +72,7 @@ Lemma wp_lift_atomic_head_step_fupd {s E1 E2 Φ} e1 :
     ∀ e2 σ2 efs, ⌜head_step e1 σ1 κ e2 σ2 efs⌝ ={E1,E2}▷=∗
       state_interp σ2 κs (length efs + n) ∗
       from_option Φ False (to_val e2) ∗
-      [∗ list] ef ∈ efs, WP ef @ s; ⊤ {{ _, fork_post }})
+      [∗ list] ef ∈ efs, WP ef @ s; ⊤ {{ fork_post }})
   ⊢ WP e1 @ s; E1 {{ Φ }}.
 Proof.
   iIntros (?) "H". iApply wp_lift_atomic_step_fupd; [done|].
@@ -88,7 +88,7 @@ Lemma wp_lift_atomic_head_step {s E Φ} e1 :
     ▷ ∀ e2 σ2 efs, ⌜head_step e1 σ1 κ e2 σ2 efs⌝ ={E}=∗
       state_interp σ2 κs (length efs + n) ∗
       from_option Φ False (to_val e2) ∗
-      [∗ list] ef ∈ efs, WP ef @ s; ⊤ {{ _, fork_post }})
+      [∗ list] ef ∈ efs, WP ef @ s; ⊤ {{ fork_post }})
   ⊢ WP e1 @ s; E {{ Φ }}.
 Proof.
   iIntros (?) "H". iApply wp_lift_atomic_step; eauto.
