theories/program_logic/total_lifting.v
@@ -21,7 +21,7 @@ Lemma twp_lift_step s E Φ e1 :
       ⌜κ = []⌝ ∗
       state_interp σ2 κs (length efs + n) ∗
       WP e2 @ s; E [{ Φ }] ∗
-      [∗ list] ef ∈ efs, WP ef @ s; ⊤ [{ _, fork_post }])
+      [∗ list] ef ∈ efs, WP ef @ s; ⊤ [{ fork_post }])
   ⊢ WP e1 @ s; E [{ Φ }].
 Proof. by rewrite twp_unfold /twp_pre=> ->. Qed.
 
@@ -52,7 +52,7 @@ Lemma twp_lift_atomic_step {s E Φ} e1 :
       ⌜κ = []⌝ ∗
       state_interp σ2 κs (length efs + n) ∗
       from_option Φ False (to_val e2) ∗
-      [∗ list] ef ∈ efs, WP ef @ s; ⊤ [{ _, fork_post }])
+      [∗ list] ef ∈ efs, WP ef @ s; ⊤ [{ fork_post }])
   ⊢ WP e1 @ s; E [{ Φ }].
 Proof.
   iIntros (?) "H".
